Finished updating Mulx CorrectnessProof

proof/crypto_scalarmult/curve25519/amd64/mulx/CorrectnessProof.ec
@@ -1,200 +1,686 @@
-require import AllCore Bool List Int IntExtra IntDiv CoreMap Real Zp.
-from Jasmin require import JModel.
-require import Curve25519_Spec.
-require import Curve25519_Hop1.
-require import Curve25519_Hop2.
-require import Curve25519_Hop3.
-require import Curve25519_smulx.
-import Zp ZModpRing.
-import Curve25519_Spec Curve25519_Hop1 Curve25519_Hop2 Curve25519_Hop3.
-import Curve25519_smulx.
+require import AllCore Bool List Int IntDiv StdOrder CoreMap Real Ring Distr Zp.
+from Jasmin require import JModel JMemory JWord JWord_array JUtils.
+require import Curve25519_Procedures.
+require import Curve25519_Operations.
+require import Scalarmult_s.
+import Zp Zp_25519 Zp_limbs.
+import Curve25519_Procedures Curve25519_Operations StdOrder.IntOrder EClib.
+import Scalarmult_s.
 
-require import Array4 Array8.
+require import Array4 Array8 Array32.
 require import W64limbs.
 
-(** representation : move to another file/use rep3/5 **)
-type Rep4 = W64.t Array4.t.
-op valRep4  (x : Rep4) : int = val_limbs64 (to_list x).
-op inzpRep4 (x : Rep4) : zp  = inzp (valRep4 x) axiomatized by inzpRep4E.
-abbrev zpcgrRep4 (x : Rep4) (z : int) : bool = zpcgr (valRep4 x) z.
-(** ************************************* **)
+abbrev zexp = ZModpRing.exp.
+
+(** hoares, lossless and phoares **)
+lemma h_add_rrs_mulx (_f _g: zp):
+  hoare [M.__add4_rrs :
+      inzpRep4 f = _f /\ inzpRep4 g = _g
+      ==>
+      inzpRep4 res = _f + _g
+  ].
+proof.
+    proc.
+    admit.
+qed.
+
+lemma h_sub_rrs_mulx (_f _g: zp):
+  hoare [M.__sub4_rrs :
+      inzpRep4 f = _f /\ inzpRep4 gs = _g
+      ==>
+      inzpRep4 res = _f - _g
+  ].
+proof.
+    proc.
+    admit.
+qed.
+
+(* inline mul4_c0 mul4_c1 mul4_c2 mul4_c3 *)
+
+lemma h_mul_a24_mulx (_f : zp, _a24: int):
+  hoare [M.__mul4_a24_rs :
+      inzpRep4 fs = _f /\  _a24 = to_uint a24
+      ==>
+      inzpRep4 res = _f * inzp _a24
+  ].
+proof.
+    proc.
+    admit.
+qed.
+
+
+lemma h_mul_rsr_mulx (_f _g: zp):
+  hoare [M.__mul4_rsr :
+      inzpRep4 fs = _f /\  inzpRep4 g = _g
+      ==>
+      inzpRep4 res = _f * _g
+  ].
+proof.
+    proc.
+    admit.
+qed.
+
+lemma h_sqr_rr_mulx (_f: zp):
+  hoare [M.__sqr4_rr :
+      inzpRep4 f = _f
+      ==>
+      inzpRep4 res = ZModpRing.exp _f 2
+  ].
+proof.
+    proc.
+    admit.
+qed.
+
+lemma ill_add_rrs_mulx : islossless M.__add4_rrs.
+    by proc; do 2! unroll for ^while; islossless.
+qed.
+
+lemma ph_add_rrs_mulx (_f _g: zp):
+    phoare [M.__add4_rrs :
+      inzpRep4 f = _f /\ inzpRep4 g = _g
+      ==>
+      inzpRep4 res = _f + _g
+  ] = 1%r.
+proof.
+    by conseq ill_add_rrs_mulx (h_add_rrs_mulx _f _g).
+qed.
+
+lemma ill_sub_rrs_mulx : islossless M.__sub4_rrs.
+    by proc; do 2! unroll for ^while; islossless.
+qed.
+
+lemma ph_sub_rrs_mulx (_f _g: zp):
+    phoare [M.__sub4_rrs :
+      inzpRep4 f = _f /\ inzpRep4 gs = _g
+      ==>
+      inzpRep4 res = _f - _g
+  ] = 1%r.
+proof.
+    by conseq ill_sub_rrs_mulx (h_sub_rrs_mulx _f _g).
+qed.
+
+lemma ill_mul_a24_mulx : islossless M.__mul4_a24_rs by islossless.
+
+lemma ph_mul_a24_mulx (_f: zp, _a24: int):
+    phoare [M.__mul4_a24_rs :
+      inzpRep4 fs = _f /\  _a24 = to_uint a24
+      ==>
+      inzpRep4 res = _f * inzp _a24
+  ] = 1%r.
+proof.
+    by conseq ill_mul_a24_mulx (h_mul_a24_mulx _f _a24).
+qed.
+
+lemma ill_mul_rsr_mulx : islossless M.__mul4_rsr by islossless.
+
+lemma ph_mul_rsr_mulx (_f _g : zp):
+    phoare [M.__mul4_rsr :
+      inzpRep4 fs = _f /\  inzpRep4 g = _g
+      ==>
+      inzpRep4 res = _f * _g] = 1%r.
+proof.
+    by conseq ill_mul_rsr_mulx (h_mul_rsr_mulx _f _g).
+qed.
+
+lemma ill_sqr_rr_mulx : islossless M.__sqr4_rr
+    by islossless.
+
+lemma ph_sqr_rr_mulx (_f: zp):
+    phoare [M.__sqr4_rr :
+      inzpRep4 f = _f
+      ==>
+      inzpRep4 res = ZModpRing.exp _f 2] = 1%r.
+proof.
+    by conseq ill_sqr_rr_mulx (h_sqr_rr_mulx _f).
+qed.
 
 (** step 0 : add sub mul sqr **)
-equiv eq_h4_add : MHop2.add ~ M._fe64_add_rrs:
+equiv eq_spec_impl_add_rrs_mulx : CurveProcedures.add ~ M.__add4_rrs:
    f{1} = inzpRep4 f{2} /\
    g{1} = inzpRep4 g{2}
     ==>
    res{1} = inzpRep4 res{2}.
 proof.
-proc.
-admit.
+    proc *.
+    ecall {2} (ph_add_rrs_mulx (inzpRep4 f{2}) (inzpRep4 g{2})).
+    inline *; wp; skip => />.
+    move => &2 H H0 => />. by rewrite H0.
 qed.
 
-equiv eq_h4_sub : MHop2.sub ~ M._fe64_sub_rrs:
+equiv eq_spec_impl_sub_rrs_mulx : CurveProcedures.sub ~ M.__sub4_rrs:
    f{1} = inzpRep4 f{2} /\
    g{1} = inzpRep4 gs{2}
     ==>
    res{1} = inzpRep4 res{2}.
 proof.
-proc.
-admit.
+    proc *.
+    ecall {2} (ph_sub_rrs_mulx (inzpRep4 f{2}) (inzpRep4 gs{2})).
+    inline *; wp; skip => />.
+    move => &2 H H0 => />. by rewrite H0.
 qed.
 
-equiv eq_h4_mul_a24 : MHop2.mul_a24 ~ M._fe64_mul_a24:
+equiv eq_spec_impl_mul_a24_mulx : CurveProcedures.mul_a24 ~ M.__mul4_a24_rs:
    f{1} = inzpRep4 fs{2} /\
    a24{1} = to_uint a24{2}
     ==>
    res{1} = inzpRep4 res{2}.
 proof.
-proc.
-admit.
+    proc *.
+    ecall {2} (ph_mul_a24_mulx (inzpRep4 fs{2}) (to_uint a24{2})).
+    inline *; wp; skip => />.
+    move => &2 H H0 => />. by rewrite H0.
 qed.
 
-equiv eq_h4_mul : MHop2.mul ~ M._fe64_mul_rsr:
+equiv eq_spec_impl_mul_rsr_mulx : CurveProcedures.mul ~ M.__mul4_rsr:
    f{1} = inzpRep4 fs{2} /\
    g{1} = inzpRep4 g{2}
     ==>
    res{1} = inzpRep4 res{2}.
 proof.
-proc.
-admit.
+    proc *.
+    ecall {2} (ph_mul_rsr_mulx (inzpRep4 fs{2}) (inzpRep4 g{2})).
+    inline *; wp; skip => />.
+    move => &2 H H0 => />. by rewrite H0.
 qed.
 
-equiv eq_h4_sqr : MHop2.sqr ~ M._fe64_sqr_rr:
+equiv eq_spec_impl__sqr_rr_mulx : CurveProcedures.sqr ~ M.__sqr4_rr:
     f{1} = inzpRep4 f{2}
     ==>
     res{1} = inzpRep4 res{2}.
 proof.
-proc.
-admit.
+    proc *.
+    ecall {2} (ph_sqr_rr_mulx (inzpRep4 f{2})).
+    inline *; wp; skip => />.
+    move => &2 H H0 => />. by rewrite H0.
 qed.
 
 (** step 0.5 : transitivity stuff **)
-equiv eq_h4_add_ssr : MHop2.add ~ M._fe64_add_ssr:
-   f{1} = inzpRep4 fs{2} /\
-   g{1} = inzpRep4 g{2}
+equiv eq_spec_impl_add_ssr_mulx : CurveProcedures.add ~ M.__add4_ssr:
+   g{1} = inzpRep4 fs{2} /\
+   f{1} = inzpRep4 g{2}
     ==>
    res{1} = inzpRep4 res{2}.
 proof.
-proc.
-admit.
+    proc *. inline M.__add4_ssr. wp. sp.
+    call eq_spec_impl_add_rrs_mulx. skip. auto => />.
 qed.
 
-equiv eq_h4_add_sss : MHop2.add ~ M._fe64_add_sss:
-   f{1} = inzpRep4 fs{2} /\
-   g{1} = inzpRep4 gs{2}
-    ==>
-   res{1} = inzpRep4 res{2}.
-proof.
-proc.
-admit.
-qed.
-
-equiv eq_h4_sub_ssr : MHop2.sub ~ M._fe64_sub_ssr:
-   f{1} = inzpRep4 fs{2} /\
-   g{1} = inzpRep4 g{2}
-    ==>
-   res{1} = inzpRep4 res{2}.
-proof.
-proc.
-admit.
-qed.
-
-equiv eq_h4_sub_sss : MHop2.sub ~ M._fe64_sub_sss:
+equiv eq_spec_impl_add_sss_mulx : CurveProcedures.add ~ M.__add4_sss:
    f{1} = inzpRep4 fs{2} /\
    g{1} = inzpRep4 gs{2}
     ==>
    res{1} = inzpRep4 res{2}.
 proof.
-proc.
-admit.
+    proc *. inline M.__add4_sss. wp. sp.
+    call eq_spec_impl_add_rrs_mulx. skip. auto => />.
 qed.
 
-equiv eq_h4_mul_a24_ss : MHop2.mul_a24 ~ M._fe64_mul_a24_ss:
+equiv eq_spec_impl_sub_ssr_mulx : CurveProcedures.sub ~ M.__sub4_ssr:
+   f{1} = inzpRep4 fs{2} /\
+   g{1} = inzpRep4 g{2}
+    ==>
+   res{1} = inzpRep4 res{2}.
+proof.
+    proc *. inline M.__sub4_ssr. wp. sp.
+    call eq_spec_impl_sub_rsr_mulx. skip. auto => />.
+qed.
+
+equiv eq_spec_impl_sub_sss_mulx : CurveProcedures.sub ~ M.__sub4_sss:
+   f{1} = inzpRep4 fs{2} /\
+   g{1} = inzpRep4 gs{2}
+    ==>
+   res{1} = inzpRep4 res{2}.
+proof.
+    proc *.  inline M.__sub4_sss. wp. sp.
+    call eq_spec_impl_sub_rrs_mulx. skip. auto => />.
+qed.
+
+equiv eq_spec_impl_mul_a24_ss_mulx : CurveProcedures.mul_a24 ~ M.__mul4_a24_ss:
    f{1} = inzpRep4 fs{2} /\
    a24{1} = to_uint a24{2}
     ==>
    res{1} = inzpRep4 res{2}.
 proof.
-proc.
-admit.
+    proc *.  inline M.__mul4_a24_ss. wp. sp.
+    call eq_spec_impl_mul_a24_mulx. skip. auto => />.
 qed.
 
-equiv eq_h4_mul_rss : MHop2.mul ~ M._fe64_mul_rss:
+equiv eq_spec_impl_mul_rss_mulx : CurveProcedures.mul ~ M.__mul4_rss:
    f{1} = inzpRep4 fs{2} /\
    g{1} = inzpRep4 gs{2}
     ==>
    res{1} = inzpRep4 res{2}.
 proof.
-proc.
-admit.
+    proc *. inline M.__mul4_rss. wp. sp.
+    call eq_spec_impl_mul_rsr_mulx. skip. auto => />.
 qed.
 
-equiv eq_h4_mul_ssr : MHop2.mul ~ M._fe64_mul_ssr:
+equiv eq_spec_impl_mul_ssr_mulx : CurveProcedures.mul ~ M.__mul4_ssr:
    f{1} = inzpRep4 fs{2} /\
    g{1} = inzpRep4 g{2}
     ==>
    res{1} = inzpRep4 res{2}.
 proof.
-proc.
-admit.
+    proc *. inline M.__mul4_ssr. wp. sp.
+    call eq_spec_impl_mul_rsr_mulx. skip. auto => />.
 qed.
 
-equiv eq_h4_mul_sss : MHop2.mul ~ M._fe64_mul_sss:
+equiv eq_spec_impl_mul_sss_mulx : CurveProcedures.mul ~ M.__mul4_sss:
    f{1} = inzpRep4 fs{2} /\
    g{1} = inzpRep4 gs{2}
     ==>
    res{1} = inzpRep4 res{2}.
 proof.
-proc.
-admit.
+    proc *. inline M.__mul4_sss. wp. sp.
+    call eq_spec_impl_mul_rsr_mulx. skip. auto => />.
 qed.
 
-equiv eq_h4_sqr_rs : MHop2.sqr ~ M._fe64_sqr_rs:
+equiv eq_spec_impl_sqr_rs_mulx : CurveProcedures.sqr ~ M.__sqr4_rs:
     f{1} = inzpRep4 fs{2}
     ==>
     res{1} = inzpRep4 res{2}.
 proof.
-proc.
-admit.
+    proc *.  inline M.__sqr4_rs. wp. sp.
+    call eq_spec_impl__sqr_rr_mulx. skip. auto => />.
 qed.
 
-equiv eq_h4_sqr_ss : MHop2.sqr ~ M._fe64_sqr_ss:
+equiv eq_spec_impl_sqr_ss_mulx : CurveProcedures.sqr ~ M.__sqr4_ss:
     f{1} = inzpRep4 fs{2}
     ==>
     res{1} = inzpRep4 res{2}.
 proof.
-proc.
-admit.
+    proc *.  inline M.__sqr4_ss. wp. sp.
+    call eq_spec_impl__sqr_rr_mulx. skip. auto => />.
 qed.
+
+equiv eq_spec_impl_mul_rsr__rpr_mulx : M.__mul4_rsr ~ M.__mul4_rpr:
+    fs{1}   = fp{2} /\
+    g{1}   =  g{2}
+    ==>
+    res{1} = res{2}.
+proof.
+    by sim.
+qed.
+
+equiv eq_spec_impl_mul__rpr_mulx : CurveProcedures.mul ~ M.__mul4_rpr:
+   f{1}   = inzpRep4 fp{2} /\
+   g{1}   = inzpRep4 g{2}
+   ==>
+   res{1} = inzpRep4 res{2}.
+proof.
+    transitivity
+    M.__mul4_rsr
+    ( f{1} = inzpRep4 fs{2} /\ g{1} = inzpRep4 g{2} ==> res{1} = inzpRep4 res{2})
+    ( fs{1} = fp{2} /\ g{1} = g{2} ==> res{1} = res{2}).
+    move => &1 &2 [H] H0.
+    exists(fp{2}, g{2}) => />.
+    move => &1 &m &2 => H H0. by rewrite -H0 H.
+    proc *; call eq_spec_impl_mul_rsr_mulx.
+    by skip => />.
+    proc *; call eq_spec_impl_mul_rsr__rpr_mulx.
+    by done.
+qed.
+
+equiv eq_spec_impl_sub_rrs_rsr_mulx : M.__sub4_rrs ~ M.__sub4_rsr:
+    f{1} = fs{2} /\ gs{1} = g{2} ==> ={res}.
+proof.
+    proc.
+    do 2! unroll for{1} ^while.
+    do 2! unroll for{2} ^while.
+    wp; skip => />.
+qed.
+
+equiv eq_spec_impl_sub_rsr_mulx : CurveProcedures.sub ~ M.__sub4_rsr:
+   f{1}   = inzpRep4 fs{2} /\
+   g{1}   = inzpRep4 g{2}
+   ==>
+   res{1} = inzpRep4 res{2}.
+proof.
+    transitivity
+    M.__sub4_rrs
+    ( f{1} = inzpRep4 f{2} /\ g{1} = inzpRep4 gs{2} ==> res{1} = inzpRep4 res{2})
+    ( f{1} = fs{2} /\ gs{1} = g{2} ==> res{1} = res{2}).
+    move => &1 &2 [H] H0.
+    exists(fs{2}, g{2}) => />.
+    move => &1 &m &2 H H0. by rewrite -H0 H.
+    proc *; call eq_spec_impl_sub_rrs_mulx.
+    by skip => />.
+    proc *; call eq_spec_impl_sub_rrs_rsr_mulx.
+    by done.
+qed.
+
+equiv eq_spec_impl_mul_rpr_mulx : CurveProcedures.mul ~ M._mul4_rpr:
+    f{1}   = inzpRep4 fp{2} /\
+    g{1}   = inzpRep4 g{2}
+    ==>
+    res{1} = inzpRep4 res{2}.
+proof.
+    proc *.  inline M._mul4_rpr. wp. sp.
+    call eq_spec_impl_mul__rpr_mulx. skip. auto => />.
+qed.
+
+equiv eq_spec_impl_mul_rsr__mulx : CurveProcedures.mul ~ M._mul4_rsr_:
+    f{1}   = inzpRep4 _fs{2} /\
+    g{1}   = inzpRep4 _g{2}
+    ==>
+    res{1} = inzpRep4 res{2}.
+proof.
+    proc *.  inline M._mul4_rsr_. wp. sp.
+    call eq_spec_impl_mul_rpr_mulx. skip. auto => />.
+qed.
+
+equiv eq_spec_impl_sqr_rr_mulx : CurveProcedures.sqr ~ M._sqr4_rr:
+    f{1}   = inzpRep4 f{2}
+    ==>
+    res{1} = inzpRep4 res{2}.
+proof.
+    proc *.  inline M._sqr4_rr. wp. sp.
+    call (eq_spec_impl__sqr_rr_mulx) . skip. auto => />.
+qed.
+
+
+equiv eq_spec_impl_sqr_rr__mulx : CurveProcedures.sqr ~ M._sqr4_rr_:
+    f{1}   = inzpRep4 _f{2}
+    ==>
+    res{1} = inzpRep4 res{2}.
+proof.
+    proc *. inline M._sqr4_rr_. wp. sp. rewrite /copy_64 => />.
+    call eq_spec_impl_sqr_rr_mulx. skip. auto => />.
+qed.
+
+(** setting last bit to 0 **)
+lemma eq_set_last_bit_to_zero64_mulx x :
+  hoare [
+      M.__decode_u_coordinate4 :
+      u = x
+      ==>
+      res = Curve25519_Operations.last_bit_to_zero64 x
+  ].
+proof.
+    proc; wp; skip => />.
+    rewrite /last_bit_to_zero64 => />; congr.
+    pose X := x.[3].
+    rewrite /of_int /int2bs  /mkseq /to_list -iotaredE => />.
+    rewrite andE  wordP => /> k K0 K1.
+    rewrite  map2iE //  get_bits2w //.
+    smt(W64.initE).
+qed.
+
+lemma ill_set_last_bit_to_zero64_mulx: islossless M.__decode_u_coordinate4 by islossless.
+
+lemma eq_ph_set_last_bit_to_zero64_mulx x:
+  phoare [
+    M.__decode_u_coordinate4 :
+    u = x
+    ==>
+    res = Curve25519_Operations.last_bit_to_zero64 x
+  ] = 1%r.
+proof.
+    by conseq ill_set_last_bit_to_zero64_mulx (eq_set_last_bit_to_zero64_mulx x).
+qed.
+
+(** to bytes **)
+lemma eq_to_bytes_mulx r:
+  hoare [M.__tobytes4 :
+      r = f
+      ==>
+      pack4 (to_list res) = (W256.of_int (asint (inzpRep4 r)))
+  ].
+proof.
+    proc.
+    admit.
+qed.
+
+lemma ill_to_bytes_mulx : islossless M.__tobytes4 by islossless.
+
+lemma ph_to_bytes_mulx r:
+  phoare [M.__tobytes4 :
+      r = f
+      ==>
+      pack4 (to_list res) = (W256.of_int (asint (inzpRep4 r)))
+  ] = 1%r.
+proof.
+    by conseq ill_to_bytes_mulx (eq_to_bytes_mulx r).
+qed.
+
 
 (** step 1 : decode_scalar_25519 **)
-equiv eq_h4_decode_scalar_25519 :
-  MHop2.decode_scalar_25519 ~ M.decode_scalar_25519:
-  true ==> true.
+equiv eq_spec_impl_decode_scalar_25519_mulx : CurveProcedures.decode_scalar ~ M.__decode_scalar:
+  k'{1}  = pack4 (to_list k{2})
+    ==>
+    res{1} = pack32 (to_list res{2}).
 proof.
-admit.
+    proc; wp; auto => />.
+    unroll for{2} ^while => />; wp; skip => /> &2.
+    rewrite !/set64_direct !/get8 !/init8 => />.
+    rewrite pack4E pack32E.
+    rewrite !/to_list /mkseq -!iotaredE => /> .
+    rewrite !of_intE modz_small. by apply bound_abs. rewrite !bits2wE /int2bs /mkseq -!iotaredE => />.
+    rewrite wordP => i rgi />.
+    rewrite !of_listE !bits8E //= => />.
+    rewrite !get_setE //= !orE !andE !map2E //=.
+    rewrite !initiE => />.
+    rewrite !initiE => />. smt(). smt().
+    + case(i = 0) => /> *; case(i = 1) => /> *; case(i = 2) => /> *; case(i = 254) => /> *; case(i = 255) => /> *.
+    + case(i %/ 8 = 0) => /> *.
+    + rewrite initiE => /> . smt(). rewrite initiE => />. smt(). rewrite initiE => />. smt(). smt().
+    + case(i %/ 8 - 1 = 0) => /> *.
+    + rewrite initiE => /> /#.
+    + case(i %/ 8 - 2 = 0) => /> *.
+    + rewrite initiE => /> /#.
+    + case(i %/ 8 - 3 = 0) => /> *.
+    + rewrite initiE => /> /#.
+    + case(i %/ 8 - 4 = 0) => /> *.
+    rewrite initiE => /> /#.
+    + case(i %/ 8 - 5 = 0) => /> *.
+    + rewrite initiE => /> /#.
+    + case(i %/ 8 - 6 = 0) => /> *.
+    + rewrite initiE => /> /#.
+    + case(i %/ 8 - 7 = 0) => /> *.
+    + rewrite initiE => /> /#.
+    + case(i %/ 8 - 8 = 0) => /> *.
+    + rewrite initiE => /> /#.
+    + case(i %/ 8 - 9 = 0) => /> *.
+    + rewrite initiE => /> /#.
+    + case(i %/ 8 - 10 = 0) => /> *.
+    + rewrite initiE => /> /#.
+    + case(i %/ 8 - 11 = 0) => /> *.
+    + rewrite initiE => /> /#.
+    + case(i %/ 8 - 12 = 0) => /> *.
+    + rewrite initiE => /> /#.
+    + case(i %/ 8 - 13 = 0) => /> *.
+    + rewrite initiE => /> /#.
+    + case(i %/ 8 - 14 = 0) => /> *.
+    + rewrite initiE => /> /#.
+    + case(i %/ 8 - 15 = 0) => /> *.
+    + rewrite initiE => /> /#.
+    + case(i %/ 8 - 16 = 0) => /> *.
+    + rewrite initiE => /> /#.
+    + case(i %/ 8 - 17 = 0) => /> *.
+    + rewrite initiE => /> /#.
+    + case(i %/ 8 - 18 = 0) => /> *.
+    + rewrite initiE => /> /#.
+    + case(i %/ 8 - 19 = 0) => /> *.
+    + rewrite initiE => /> /#.
+    + case(i %/ 8 - 20 = 0) => /> *.
+    + rewrite initiE => /> /#.
+    + case(i %/ 8 - 21 = 0) => /> *.
+    + rewrite initiE => /> /#.
+    + case(i %/ 8 - 22 = 0) => /> *.
+    + rewrite initiE => /> /#.
+    + case(i %/ 8 - 23 = 0) => /> *.
+    + rewrite initiE => /> /#.
+    + case(i %/ 8 - 24 = 0) => /> *.
+    + rewrite initiE => /> /#.
+    + case(i %/ 8 - 25 = 0) => /> *.
+    + rewrite initiE => /> /#.
+    + case(i %/ 8 - 26 = 0) => /> *.
+    + rewrite initiE => /> /#.
+    + case(i %/ 8 - 27 = 0) => /> *.
+    + rewrite initiE => /> /#.
+    + case(i %/ 8 - 28 = 0) => /> *.
+    + rewrite initiE => /> /#.
+    + case(i %/ 8 - 29 = 0) => /> *.
+    + rewrite initiE => /> /#.
+    + case(i %/ 8 - 30 = 0) => /> *.
+    + rewrite initiE => /> /#.
+    + case(i %/ 8 - 31 = 0) => /> *.
+    + rewrite !initiE => />. smt().
+    + rewrite !initiE => />. smt().
+    case(i %/ 64 = 0) => /> *. smt(). smt().
+    + rewrite !initiE => /> /#. smt().
 qed.
 
 (** step 2 : decode_u_coordinate **)
-equiv eq_h4_decode_u_coordinate :
-  MHop2.decode_u_coordinate ~ M.decode_u_coordinate:
-  true ==> true.
+equiv eq_spec_impl_decode_u_coordinate_mulx : CurveProcedures.decode_u_coordinate ~ M.__decode_u_coordinate4:
+  u'{1}                      =     pack4 (to_list u{2})
+  ==>
+    res{1}                     =     inzpRep4 res{2}.
 proof.
-admit.
+    proc *.
+    ecall {2} (eq_ph_set_last_bit_to_zero64_mulx u{2}).
+    inline *; wp; skip => /> &2.
+    rewrite inzpRep4E. congr.
+    rewrite to_uint_unpack4u64  valRep4E; congr; congr.
+    rewrite /last_bit_to_zero64 => />.
+    rewrite /to_list /mkseq /to_list -iotaredE => />.
+    do split.
+    + rewrite !wordP => /> i I I0. rewrite !bits64iE => />.
+    + rewrite set_neqiE. smt().
+    + rewrite pack4E => />. rewrite of_listE => />.
+    + rewrite initE => />.
+    + have ->: (0 <= i && i < 256) by smt(). auto => />.
+    + rewrite initE => />. have ->: 0 <= i %/ 64 by smt(). auto => />.
+    + case(i %/ 64 < 4) => /> *. smt(). smt().
+    + rewrite !wordP => /> i I I0. rewrite !bits64iE => />.
+    + rewrite set_neqiE. smt().
+    + rewrite pack4E => />. rewrite of_listE => />.
+    + rewrite initE => />.
+    + have ->: (0 <= 64 + i && 64 + i < 256) by smt(). auto => />.
+    + rewrite initE => />. have ->: 0 <= (64 + i) %/ 64 by smt(). auto => />.
+    + case((64 + i) %/ 64 < 4) => /> *. smt(). smt().
+    + rewrite !wordP => /> i I I0. rewrite !bits64iE => />.
+    + rewrite set_neqiE. smt().
+    + rewrite pack4E => />. rewrite of_listE => />.
+    + rewrite initE => />.
+    + have ->: (0 <= 128 + i && 128 + i < 256) by smt(). auto => />.
+    + rewrite initE => />. have ->: 0 <= (128 + i) %/ 64 by smt(). auto => />.
+    + case((128 + i) %/ 64 < 4) => /> *. smt(). smt().
+    + rewrite !wordP => /> i I I0. rewrite !bits64iE => />.
+    rewrite pack4E => />. rewrite of_listE => />.
+    rewrite !setE => />. rewrite initE => />.
+    have ->: (0 <= 192 + i && 192 + i < 256) by smt(). auto => />.
+    rewrite !initE => />.
+    have ->: (0 <= i && i < 64) by smt().
+    have ->: (0 <= 192 + i && 192 + i < 256) by smt().
+    auto => />.
+    case (i <> 63) => /> C.
+    have ->: 192 + i <> 255 by smt().
+    auto => />. rewrite !initE. smt().
 qed.
+
+equiv eq_spec_impl_decode_u_coordinate_base_mulx :
+    CurveProcedures.decode_u_coordinate_base ~ M.__decode_u_coordinate_base4:
+        true
+        ==>
+        res{1} = inzpRep4 res{2}.
+proof.
+    proc *.
+    inline *; wp; skip => />.
+    rewrite inzpRep4E. congr.
+    rewrite to_uint_unpack4u64  valRep4E; congr; congr.
+    rewrite /last_bit_to_zero64 => />.
+    have !->: ((of_int 9))%W256.[255 <- false] = ((of_int 9))%W256.
+    rewrite !of_intE !bits2wE !/int2bs !/mkseq -iotaredE => />.
+    apply W256.ext_eq => />. move => X X0 X1.
+    rewrite get_setE //. case (X = 255) => /> C.
+    rewrite /to_list /mkseq /to_list -iotaredE => />.
+qed.
+
 
 (** step 3 : ith_bit **)
-equiv eq_h4_ith_bit :
-  MHop2.ith_bit ~ M.ith_bit:
-  true ==> true.
+equiv eq_spec_impl_ith_bit_mulx : CurveProcedures.ith_bit ~ M.__ith_bit :
+    k'{1} =     pack32 (to_list k{2}) /\
+    ctr{1}                   = to_uint ctr{2} /\
+    0 <= ctr{1} < 256
+    ==>
+    b2i res{1}                = to_uint res{2}.
 proof.
-admit.
+    proc; wp; skip => /> &2 H H0.
+    rewrite (W64.and_mod 3 ctr{2}) //=  (W64.and_mod 6 (of_int (to_uint ctr{2} %% 8))%W64) //= !to_uint_shr //= !shr_shrw.
+    smt(W64.to_uint_cmp  W64.of_uintK W64.to_uintK).
+    rewrite /zeroextu64 /truncateu8 //=  !of_uintK => />.
+    + rewrite  of_intE modz_small.  apply bound_abs. smt(W8.to_uint_cmp  @JUtils).
+    rewrite bits2wE /int2bs /mkseq -iotaredE => />.
+    auto => />.
+    rewrite (modz_small (to_uint ctr{2} %% 8) W64.modulus). apply bound_abs. smt(W64.to_uint_cmp).
+    rewrite (modz_small (to_uint ctr{2} %% 8) 64). apply bound_abs. smt(W64.to_uint_cmp).
+    rewrite (modz_small (to_uint ctr{2} %% 8) W64.modulus). apply bound_abs. smt(W64.to_uint_cmp).
+    pose ctr := to_uint ctr{2}.
+    rewrite pack32E of_listE /to_list !/mkseq !initiE // -!iotaredE => />.
+    rewrite !initiE //=. auto => />. smt().
+    rewrite !/b2i !of_intE !bits2wE !/int2bs !/mkseq //=.
+    rewrite -!iotaredE => />.
+    rewrite !to_uintE !/bs2int !/w2bits !/mkseq /big /range !/predT -!iotaredE => />.
+    rewrite !b2i0 => />.
+    rewrite !initiE => />. smt(). auto => />.
+    + case(ctr %/ 8 = 0) => /> *. smt().
+    + case(ctr %/ 8 - 1 = 0) => /> *. smt().
+    + case(ctr %/ 8 - 2 = 0) => /> *. smt().
+    + case(ctr %/ 8 - 3 = 0) => /> *. smt().
+    + case(ctr %/ 8 - 4 = 0) => /> *. smt().
+    + case(ctr %/ 8 - 5 = 0) => /> *. smt().
+    + case(ctr %/ 8 - 6 = 0) => /> *. smt().
+    + case(ctr %/ 8 - 7 = 0) => /> *. smt().
+    + case(ctr %/ 8 - 8 = 0) => /> *. smt().
+    + case(ctr %/ 8 - 9 = 0) => /> *. smt().
+    + case(ctr %/ 8 - 10 = 0) => /> *. smt().
+    + case(ctr %/ 8 - 11 = 0) => /> *. smt().
+    + case(ctr %/ 8 - 12 = 0) => /> *. smt().
+    + case(ctr %/ 8 - 13 = 0) => /> *. smt().
+    + case(ctr %/ 8 - 14 = 0) => /> *. smt().
+    + case(ctr %/ 8 - 15 = 0) => /> *. smt().
+    + case(ctr %/ 8 - 16 = 0) => /> *. smt().
+    + case(ctr %/ 8 - 17 = 0) => /> *. smt().
+    + case(ctr %/ 8 - 18 = 0) => /> *. smt().
+    + case(ctr %/ 8 - 19 = 0) => /> *. smt().
+    + case(ctr %/ 8 - 20 = 0) => /> *. smt().
+    + case(ctr %/ 8 - 21 = 0) => /> *. smt().
+    + case(ctr %/ 8 - 22 = 0) => /> *. smt().
+    + case(ctr %/ 8 - 23 = 0) => /> *. smt().
+    + case(ctr %/ 8 - 24 = 0) => /> *. smt().
+    + case(ctr %/ 8 - 25 = 0) => /> *. smt().
+    + case(ctr %/ 8 - 26 = 0) => /> *. smt().
+    + case(ctr %/ 8 - 27 = 0) => /> *. smt().
+    + case(ctr %/ 8 - 28 = 0) => /> *. smt().
+    + case(ctr %/ 8 - 29 = 0) => /> *. smt().
+    + case(ctr %/ 8 - 30 = 0) => /> *. smt().
+    + case(ctr %/ 8 - 31 = 0) => /> *. smt().
+    + case(ctr %/ 8 - 32 = 0) => /> *. smt().
+    smt().
 qed.
 
+equiv eq_spec_impl_init_points_mulx :
+    CurveProcedures.init_points ~ M.__init_points4 :
+        init{1} = inzpRep4 initr{2}
+        ==>
+        res{1}.`1 = inzpRep4 res{2}.`1 /\
+        res{1}.`2 = inzpRep4 res{2}.`2 /\
+        res{1}.`3 = inzpRep4 res{2}.`3 /\
+        res{1}.`4 = inzpRep4 res{2}.`4.
+ proof.
+    proc.
+    wp. unroll for{2} ^while. wp. skip. move => &1 &2 H H0 H1 H2 H3 H4 H5 H6.
+    split; auto => />. rewrite /H4 /H0 /H2 /H3 /Zp.one /set0_64_ /inzpRep4 => />.
+        rewrite /valRep4 /to_list /mkseq -iotaredE => />.
+    split; auto => />. rewrite /H5  /H0 /H3 /H2 /Zp.zero /set0_64_ /inzpRep4 => />.
+        rewrite /valRep4 /to_list /mkseq -iotaredE  => />.
+    rewrite /H6  /H0 /H3 /H2 /Zp.zero /set0_64_ /inzpRep4 // /valRep4 /to_list /mkseq -iotaredE  => />.
+ qed.
+
 (** step 4 : cswap **)
-equiv eq_h4_cswap :
-  MHop2.cswap ~ M._fe64_cswap:
+equiv eq_spec_impl_cswap_mulx :
+  CurveProcedures.cswap ~ M.__cswap4:
   x2{1}         = inzpRep4 x2{2}  /\
   z2{1}         = inzpRep4 z2r{2} /\
   x3{1}         = inzpRep4 x3{2}  /\
@@ -209,29 +695,33 @@ proof.
 proc.
 do 4! unroll for{2} ^while.
 case: (toswap{1}).
-  rcondt {1} 1 => //. wp => /=; skip.
+  rcondt {1} 1 => //. wp => /=. skip.
     move => &1 &2 [#] 4!->> ??.
-    have mask_set :  (set0_64.`6 - toswap{2}) = W64.onew. rewrite /set0_64 /=. smt(@W64).
+    have mask_set :  (set0_64.`6 - toswap{2}) = W64.onew. rewrite /set0_64_ /=. smt().
     rewrite !mask_set /=.
     have lxor1 : forall (x1 x2:W64.t),  x1 `^` (x2 `^` x1) = x2.
       move=> *. rewrite xorwC -xorwA xorwK xorw0 //.
     have lxor2 : forall (x1 x2:W64.t),  x1 `^` (x1 `^` x2) = x2.
       move=> *. rewrite xorwA xorwK xor0w //. 
   rewrite !lxor1 !lxor2.
-      split. congr. apply Array4.ext_eq. smt(@Array4).
-      split. congr. apply Array4.ext_eq. smt(@Array4).
-      split. congr. apply Array4.ext_eq. smt(@Array4).
-             congr. apply Array4.ext_eq. smt(@Array4).
+      split. congr. apply Array4.ext_eq. smt(Array4.get_setE).
+      split. congr. apply Array4.ext_eq. smt(Array4.get_setE).
+      split. congr. apply Array4.ext_eq. smt(Array4.get_setE).
+        congr. apply Array4.ext_eq. rewrite /copy_64 => />. smt(Array4.get_setE).
   rcondf {1} 1 => //. wp => /=; skip.
     move => &1 &2 [#] 4!->> ??.
-    have mask_not_set :  (set0_64.`6 - toswap{2}) = W64.zero. smt(@W64).
-    rewrite !mask_not_set !andw0 !xorw0.
-    smt(@Array4).
+    have mask_not_set :  (set0_64.`6 - toswap{2}) = W64.zero. rewrite /set0_64_ => />. smt().
+    rewrite !mask_not_set !andw0 !xorw0 !/copy_64 => />.
+    do split.
+    congr. smt(Array4.initE Array4.ext_eq Array4.set_set_if).
+    congr. smt(Array4.initE Array4.ext_eq Array4.set_set_if).
+    congr. smt(Array4.initE Array4.ext_eq Array4.set_set_if).
+    congr. smt(Array4.initE Array4.ext_eq Array4.set_set_if).
 qed.
 
 (** step 5 : add_and_double **)
-equiv eq_h4_add_and_double :
-  MHop2.add_and_double ~ M.add_and_double:
+equiv eq_spec_impl_add_and_double_mulx :
+  CurveProcedures.add_and_double ~ M.__add_and_double4:
   init{1} = inzpRep4 init{2} /\
   x2{1}   = inzpRep4 x2{2}   /\
   z2{1}   = inzpRep4 z2r{2}  /\
@@ -243,123 +733,595 @@ equiv eq_h4_add_and_double :
   res{1}.`3 = inzpRep4 res{2}.`3 /\
   res{1}.`4 = inzpRep4 res{2}.`4.
 proof.
-proc => /=.
-  call eq_h4_mul_rss.
-  call eq_h4_mul_sss.
-  call eq_h4_add_sss.
-  call eq_h4_sqr_ss.
-  call eq_h4_mul_a24_ss.
-  call eq_h4_sqr_ss.
-  call eq_h4_sub_ssr.
-  call eq_h4_mul_ssr.
-  call eq_h4_sub_sss.
-  call eq_h4_add_sss.
-  call eq_h4_sqr_rs.
-  call eq_h4_sqr_ss.
-  call eq_h4_mul_sss.
-  call eq_h4_mul_sss.
-  call eq_h4_add_sss.
-  call eq_h4_sub_sss.
-  call eq_h4_add_ssr.
-  call eq_h4_sub_ssr.
-  wp. done.
+proc => /=; wp.
+  call eq_spec_impl_mul_rss_mulx; wp.
+  call eq_spec_impl_mul_sss_mulx; wp.
+  call eq_spec_impl_add_sss_mulx; wp.
+  call eq_spec_impl_sqr_ss_mulx;  wp.
+  call eq_spec_impl_mul_a24_ss_mulx; wp.
+  call eq_spec_impl_sqr_ss_mulx; wp. swap{1} 14 1.
+  call eq_spec_impl_mul_ssr_mulx; wp.
+  call eq_spec_impl_sub_ssr_mulx; wp.
+  call eq_spec_impl_sub_sss_mulx; wp.
+  call eq_spec_impl_add_sss_mulx; wp.
+  call eq_spec_impl_sqr_rs_mulx; wp.
+  call eq_spec_impl_sqr_ss_mulx; wp.
+  call eq_spec_impl_mul_sss_mulx; wp.
+  call eq_spec_impl_mul_sss_mulx; wp.
+  call eq_spec_impl_add_sss_mulx; wp.
+  call eq_spec_impl_sub_sss_mulx; wp.
+  call eq_spec_impl_add_ssr_mulx; wp.
+  call eq_spec_impl_sub_ssr_mulx; 
+  wp. skip. by done.
 qed.
 
 (** step 6 : montgomery_ladder_step **)
-equiv eq_h4_montgomery_ladder_step :
- MHop2.montgomery_ladder_step ~ M.montgomery_ladder_step:
- true ==> true.
+equiv eq_spec_impl_montgomery_ladder_step_mulx :
+ CurveProcedures.montgomery_ladder_step ~ M.__montgomery_ladder_step4:
+        k'{1} =   pack32 (to_list k{2})         /\
+        init'{1} = inzpRep4 init{2}             /\
+        x2{1} = inzpRep4 x2{2}                  /\
+        z2{1} = inzpRep4 z2r{2}                 /\
+        x3{1} = inzpRep4 x3{2}                  /\
+        z3{1} = inzpRep4 z3{2}                  /\
+        b2i swapped{1} = to_uint swapped{2}     /\
+        ctr'{1} = to_uint ctr{2}                /\
+        0 <= ctr'{1} < 256
+        ==>
+        res{1}.`1 = inzpRep4 res{2}.`1          /\
+        res{1}.`2 = inzpRep4 res{2}.`2          /\
+        res{1}.`3 = inzpRep4 res{2}.`3          /\
+        res{1}.`4 = inzpRep4 res{2}.`4          /\
+        b2i res{1}.`5 = to_uint res{2}.`5.
 proof.
-admit.
-qed.   
+    proc => /=; wp.
+    call eq_spec_impl_add_and_double_mulx. wp.
+    call eq_spec_impl_cswap_mulx. wp.
+    call eq_spec_impl_ith_bit_mulx. wp. skip.
+    move => &1 &2 [H0] [H1] [H2] [H3] [H4] [H5] [H6] H7. split.
+    auto => />. rewrite H0.
+    move => [H8 H9] H10 H11 H12 H13 H14.
+    split;  auto => />. rewrite /H14 /H13.
+    rewrite /b2i.
+    case: (swapped{1} ^^ H10).
+    move => *. smt(W64.to_uintK W64.xorw0 W64.xorwC).
+    move => *. smt(W64.ge2_modulus W64.to_uintK W64.of_uintK W64.xorwK).
+qed.
 
 (** step 7 : montgomery_ladder **)
-equiv eq_h4_montgomery_ladder :
-  MHop2.montgomery_ladder ~ M.montgomery_ladder :
-  true ==> true.
+equiv eq_spec_impl_montgomery_ladder_mulx :
+    CurveProcedures.montgomery_ladder ~ M.__montgomery_ladder4 :
+    init'{1} = inzpRep4 u{2}                     /\
+    k'{1} =  pack32 (to_list k{2})
+    ==>
+    res{1}.`1 = inzpRep4 res{2}.`1               /\
+    res{1}.`2 = inzpRep4 res{2}.`2.
 proof.
-admit.
+    proc. wp. sp.
+    unroll {1} 4.
+    rcondt {1} 4. auto => />. inline CurveProcedures.init_points.
+        wp. sp. skip. auto => />.
+    while(
+          k'{1} = pack32 (to_list  k{2})                   /\
+          ctr{1} = to_uint ctr{2}                          /\
+          -1 <= ctr{1} < 256                                /\
+          init'{1} = inzpRep4 us{2}                        /\
+          x2{1} = inzpRep4 x2{2}                           /\
+          x3{1} = inzpRep4 x3{2}                           /\
+          z2{1} = inzpRep4 z2r{2}                          /\
+          z3{1} = inzpRep4 z3{2}                           /\
+          b2i swapped{1} = to_uint swapped{2}).
+        wp. sp. call eq_spec_impl_montgomery_ladder_step_mulx. skip. auto => />.
+        move => &1 &2 ctrR H H0 H1 H2 E3. split.
+        rewrite to_uintB. rewrite uleE to_uint1 => />. smt(). rewrite to_uint1 => />.
+        smt(W64.to_uint_cmp).
+        move => H3 H4 H5 H6 H7 H8 H9 H10 H11 H12. split. smt(W64.to_uint_cmp).
+        rewrite ultE to_uintB. rewrite uleE to_uint1. smt().
+        rewrite to_uint1 to_uint0 //=. wp.
+        call eq_spec_impl_montgomery_ladder_step_mulx. wp. call eq_spec_impl_init_points_mulx. skip. done.
 qed.
 
 (** step 8 : iterated square **)
-equiv eq_h4_it_sqr :
- MHop2.it_sqr ~ M._fe64_it_sqr:
-   f{1}            =    inzpRep4 f{2} /\
-   i{1}            =    to_uint i{2}  /\
-   i{1}            <=   W64.modulus   /\
-    2              <=   i{1}          /\
-   i{1} %% 2        =   0
-   ==>
-   res{1} = inzpRep4 res{2}.`2.
+equiv eq_spec_impl_it_sqr_aux_mulx :
+ M.__it_sqr4_x2 ~ CurveProcedures.it_sqr_aux:
+        inzpRep4 f{1} = a{2} /\
+        W32.to_uint i{1} = l{2} /\
+        0 < l{2}
+      ==>
+    inzpRep4 res{1} = res{2}.
 proof.
-proc.
-  while (f{1}            =    inzpRep4 f{2}            /\ 
-         i{1}            =    to_uint i{2}             /\
-         i{1}            <=   W64.modulus              /\
-         0               <=   i{1}                     /\
-         i{1}            %%   2 = 0 /\
-         zf{2} = (i{2} = W64.zero)).
-  swap 2 3 3. wp. conseq(_: _ ==> f{1} = inzpRep4 f{2}).
-  move=> &1 &2 [#] ????? ->> ?? ??? /=.
-    rewrite /DEC_64 /rflags_of_aluop_nocf64 /ZF_of_w64 => /=.
-    progress.
-    smt(@W64). move : H1; smt(). smt(). smt(). smt(@W64). smt(@W64).
-  by do 2! call eq_h4_sqr; skip; done.
-  swap 3 4 4. wp. conseq(_: _ ==> f{1} = inzpRep4 f{2}).
-  move=> &1 &2 [#] /= ->> ->> ??? ?? ->> /=.
-    rewrite /DEC_64 /rflags_of_aluop_nocf64 /ZF_of_w64 => /=.
-    progress.
-    smt(@W64). move : H1; smt(). smt(). smt(). smt(@W64). smt(@W64).
-  by do 2! call eq_h4_sqr; wp; skip; done.
+proc; simplify.
+  while(
+        0 <= ii{2} /\ 0 <= W32.to_uint i{1} /\ ii{2} = W32.to_uint i{1} /\
+        f{2} = inzpRep4 f{1}  /\ zf{1} = (0 = W32.to_uint i{1})
+    ).
+    wp.
+    symmetry.
+    call eq_spec_impl__sqr_rr_mulx. wp. call eq_spec_impl__sqr_rr_mulx. wp. symmetry.
+    skip => />.
+    move => &1 *. do split. smt().
+    rewrite /DEC_32 /rflags_of_aluop_nocf_w => />.
+    + rewrite to_uintB. rewrite uleE to_uint1; smt(). rewrite to_uint1. smt(W32.to_uint_cmp).
+    rewrite /DEC_32 /rflags_of_aluop_nocf_w => />. rewrite to_uintB.
+    + rewrite uleE to_uint1; smt(). rewrite to_uint1 //.
+    rewrite /DEC_32 /rflags_of_aluop_nocf_w => />. rewrite /ZF_of to_uintB.
+    + rewrite uleE to_uint1. smt(). rewrite -to_uintB. rewrite uleE. smt(W32.to_uint_cmp).
+    + rewrite to_uintB. rewrite uleE to_uint1; smt(). rewrite to_uint1.
+    smt(W32.ge2_modulus W32.of_uintK W32.to_uintK W32.of_intD).
+  rewrite /DEC_32 /rflags_of_aluop_nocf_w => />. rewrite /ZF_of => *.
+  smt(W32.ge2_modulus W32.of_uintK W32.to_uintK W32.to_uintN W32.of_intD).
+    rewrite /DEC_32 /rflags_of_aluop_nocf_w => />. rewrite /ZF_of => *.
+    smt(W32.ge2_modulus W32.of_uintK W32.to_uintK W32.to_uintN W32.of_intD).
+  wp. symmetry. call eq_spec_impl__sqr_rr_mulx. wp. call eq_spec_impl__sqr_rr_mulx. wp.
+  symmetry.
+  skip => />. move => &1 H.
+  do split. smt().
+    rewrite /DEC_32 /rflags_of_aluop_nocf_w => />. rewrite /ZF_of => *.
+    smt(W32.ge2_modulus W32.of_uintK W32.to_uintK W32.to_uintN W32.of_intD).
+    rewrite /DEC_32 /rflags_of_aluop_nocf_w => />. rewrite /ZF_of => *.
+  rewrite to_uintB. rewrite uleE to_uint1. smt(W32.to_uint_cmp). rewrite to_uint1 //.
+  rewrite /DEC_32 /rflags_of_aluop_nocf_w => />. rewrite /ZF_of => *.
+ smt(W32.ge2_modulus W32.of_uintK W32.to_uintK W32.to_uintN W32.of_intD).
+rewrite /DEC_32 /rflags_of_aluop_nocf_w => />. rewrite /ZF_of => *.
+ smt(W32.ge2_modulus W32.of_uintK W32.to_uintK W32.to_uintN W32.of_intD).
+  rewrite /DEC_32 /rflags_of_aluop_nocf_w => />. rewrite /ZF_of => *.
+  smt(W32.ge2_modulus W32.of_uintK W32.to_uintK W32.to_uintN W32.of_intD).
 qed.
 
+equiv eq_spec_impl_it_sqr_aux_mulx_test :
+        CurveProcedures.it_sqr_aux ~ M.__it_sqr4_x2:
+        a{1} = inzpRep4 f{2} /\
+        l{1} = W32.to_uint i{2} /\
+        0 < l{1}
+        ==>
+        res{1} = inzpRep4 res{2}.
+proof.
+    proc; simplify.
+    while(
+        0 <= ii{1} /\ 0 <= W32.to_uint i{2} /\ ii{1} = W32.to_uint i{2} /\
+        f{1} = inzpRep4 f{2}  /\ zf{2} = (0 = W32.to_uint i{2})
+    ).
+    wp. call eq_spec_impl__sqr_rr_mulx. wp. call eq_spec_impl__sqr_rr_mulx. wp.
+    skip => />.
+    move => &1 *. do split. smt().
+    rewrite /DEC_32 /rflags_of_aluop_nocf_w => />.
+    + rewrite to_uintB. rewrite uleE to_uint1; smt(). rewrite to_uint1. smt(W32.to_uint_cmp).
+    rewrite /DEC_32 /rflags_of_aluop_nocf_w => />. rewrite to_uintB.
+    + rewrite uleE to_uint1; smt(). rewrite to_uint1 //.
+    rewrite /DEC_32 /rflags_of_aluop_nocf_w => />. rewrite /ZF_of to_uintB.
+    + rewrite uleE to_uint1. smt(). rewrite -to_uintB. rewrite uleE. smt(W32.to_uint_cmp).
+    + rewrite to_uintB. rewrite uleE to_uint1; smt(). rewrite to_uint1.
+    smt(W32.ge2_modulus W32.of_uintK W32.to_uintK W32.of_intD).
+    rewrite /DEC_32 /rflags_of_aluop_nocf_w => />. rewrite /ZF_of => *.
+    smt(W32.ge2_modulus W32.of_uintK W32.to_uintK W32.to_uintN W32.of_intD).
+    rewrite /DEC_32 /rflags_of_aluop_nocf_w => />. rewrite /ZF_of => *.
+    smt(W32.ge2_modulus W32.of_uintK W32.to_uintK W32.to_uintN W32.of_intD).
+    wp. call eq_spec_impl__sqr_rr_mulx. wp. call eq_spec_impl__sqr_rr_mulx. wp.
+    skip => />. move => &1 H.
+    do split. smt().
+    rewrite /DEC_32 /rflags_of_aluop_nocf_w => />. rewrite /ZF_of => *.
+    smt(W32.ge2_modulus W32.of_uintK W32.to_uintK W32.to_uintN W32.of_intD).
+    rewrite /DEC_32 /rflags_of_aluop_nocf_w => />. rewrite /ZF_of => *.
+    rewrite to_uintB. rewrite uleE to_uint1. smt(W32.to_uint_cmp). rewrite to_uint1 //.
+    rewrite /DEC_32 /rflags_of_aluop_nocf_w => />. rewrite /ZF_of => *.
+    smt(W32.ge2_modulus W32.of_uintK W32.to_uintK W32.to_uintN W32.of_intD).
+    rewrite /DEC_32 /rflags_of_aluop_nocf_w => />. rewrite /ZF_of => *.
+    smt(W32.ge2_modulus W32.of_uintK W32.to_uintK W32.to_uintN W32.of_intD).
+    rewrite /DEC_32 /rflags_of_aluop_nocf_w => />. rewrite /ZF_of => *.
+    smt(W32.ge2_modulus W32.of_uintK W32.to_uintK W32.to_uintN W32.of_intD).
+qed.
+
+
+lemma eq_spec_impl__it_sqr_mulx (i1: int) (i2: int):
+    i1 = i2 => 2 <= i1  =>
+equiv[
+        M.__it_sqr4_x2 ~ CurveProcedures.it_sqr:
+        i1 = W32.to_uint i{1} /\
+        i2 = i{2}   /\
+        W32.to_uint i{1} = i{2} /\
+        inzpRep4 f{1} = f{2}
+        ==>
+        inzpRep4 res{1} = zexp res{2} (exp 2 i1)
+    ].
+proof.
+    move => I I0.
+    transitivity
+     CurveProcedures.it_sqr_aux
+     (
+       l{2} = W32.to_uint i{1}  /\
+       a{2} = inzpRep4 f{1} /\
+       1 < l{2}
+        ==>
+        inzpRep4 res{1} = res{2})
+     (  a{1} = f{2} /\
+        l{1} = i{2} /\
+        l{1} = i1 /\
+        l{1} = i2 /\
+        2 <= i{2}
+        ==>
+        res{1} = zexp res{2} (exp 2 i1)).
+    auto => />.
+    move => &1 &2 *.
+    exists(f{2}, i{2}) => />. smt().
+    move => &1 &m &2 H H0. rewrite -H0. assumption.
+    proc *.
+    call eq_spec_impl_it_sqr_aux_mulx. skip => />. smt(W32.to_uint_cmp).
+
+    proc; inline *; simplify.
+    seq 7 6 : (ii{1} = l{1} - 1 /\
+        h{2} = (zexp a{1} 2) /\
+        0 <= ii{2} /\
+        0 <= ii{1} /\
+        ii{1} = ii{2} /\
+        1 <= counter{2} <= i1 /\
+        counter{2} = i1 - ii{2} /\
+        f{1} = zexp h{2} (exp 2 counter{2})).
+        wp; skip. auto => />. move => *.  smt().
+
+    while(
+        0 <= ii{1} /\
+        0 <= ii{2} /\
+        ii{1} = ii{2} /\
+        1 <= counter{2} /\
+        counter{2} = i1 - ii{2} /\
+        f{1} = zexp h{2} (exp 2 (counter{2}))).
+    wp; skip. auto => />.
+    move => &1 &2 H H0 H1.
+    smt( ZModpRing.exprM IntID.exprN IntID.exprN1 IntID.exprD_nneg).
+    skip => />. move => &1 &2 H H1 H2 H3 H4 H5 H6 H7 H8 H9.
+    have H10: H4 = 0. smt(). rewrite H10 => />.
+qed.
+
+lemma eq_spec_impl__it_sqr_mulx_x2 (i1: int) (i2: int):
+    2*i1 = i2 => 2 <= i1 => 4 <= i2 => i2 %% 2 = 0 =>
+equiv[
+        M.__it_sqr4_x2 ~ CurveProcedures.it_sqr:
+        i1 = W32.to_uint i{1} /\
+        i2 = i{2}   /\
+        2*W32.to_uint i{1} = i{2} /\
+        i{2} %% 2 = 0 /\
+        inzpRep4 f{1} = f{2}
+        ==>
+        inzpRep4 res{1} = res{2}
+    ].
+proof.
+    move => I I0 I1 I2;
+     transitivity
+     CurveProcedures.it_sqr_aux
+     (
+       l{2} = W32.to_uint i{1}  /\
+       a{2} = inzpRep4 f{1} /\
+       1 < l{2}
+        ==>
+        inzpRep4 res{1} = res{2})
+     (  a{1} = f{2} /\
+        2*l{1} = i{2} /\
+        l{1} = i1 /\
+        i{2} = i2  /\
+        4 <= i{2}  /\
+        2 <= l{1}
+        ==>
+        res{1} = res{2}).
+    auto => />. move => &1 &2 *.
+    exists(f{2}, i1) => />. smt(). smt().
+    proc *.
+    call eq_spec_impl_it_sqr_aux_mulx. skip => />. smt(W32.to_uint_cmp).
+     proc; simplify. inline *.
+     seq 7 6 : (
+        i2 = 2*l{1} /\
+        ii{1} = l{1} - counter{2} /\
+        ii{2} = i2 - counter{2} /\
+        h{2} = (zexp a{1} 2) /\
+        0 <= ii{2} /\
+        0 <= ii{1} /\
+        1 <= counter{2} <= i1 /\
+        f{1} = zexp h{2} (exp 2 counter{2})).
+    wp; skip. auto => />.
+    move => *. smt().
+      async while
+      [ (fun r => 0%r < ii%r), (ii{1} - 1)%r ]
+      [ (fun r => 0%r < ii%r), (ii{1} - 1)%r ]
+        (0 < ii{1} /\ 0 < ii{2}) (!(0 < ii{1}))
+      :
+      (
+        (ii{2} %% 2 = 0   => 2*ii{1} - 1 = ii{2})  /\
+        (ii{2} %% 2 <> 0  => 2*ii{1}     = ii{2})  /\
+        0 <= ii{1} /\
+        0 <= ii{2}
+      ).
+    auto => />;  move => &1 &2 * /#.
+    auto => />;  move => &1 &2 * /#.
+    auto => />;  move => &1 &2 * /#.
+    auto => />;  move => &2 * /#.
+    move => &1; auto => />.
+    move => v1 v2; auto => />.
+    while(
+        0 <= ii{1} /\
+        0 <= ii{2} /\
+        (ii{2} %% 2 = 0   => 2*ii{1} - 1 = ii{2})  /\
+        (ii{2} %% 2 <> 0  => 2*ii{1}     = ii{2})  /\
+        1 <= counter{2} /\
+        f{1} = zexp h{2} (exp 2 counter{2})
+    ) => //=.
+   auto => />; move => &1 &2 H H0 H1 H2 H3 H4 H5 H6 H7.
+   smt( ZModpRing.exprM IntID.exprN IntID.exprN1 IntID.exprD_nneg).
+   auto => />; move => &1 &2 H H0 H1 H2 H3 H4 H5.
+   smt( ZModpRing.exprM IntID.exprN IntID.exprN1 IntID.exprD_nneg).
+    while true (ii) => //.
+    move => H; auto => />. skip => />; move => &hr H0 H1 H2 H3 H4 H5 /#.
+    while true (ii) => //. move => H; auto => /> /#. skip => /> /#.
+    skip => />. move => &1 &2 H H0 H1 H2 H3 H4 H5 H6 H7 H8 H9 H10 H11 H12 H13 /#.
+qed.
+
+
+lemma eq_spec_impl_it_sqr_x2_mulx (i1: int) (i2: int):
+    i1 = i2 => 2 <= i1 => i2 %% 2 = 0 =>
+equiv[
+        M._it_sqr4_x2 ~ CurveProcedures.it_sqr:
+        i1 = W32.to_uint i{1} /\
+        i2 = i{2}   /\
+        W32.to_uint i{1} = i{2} /\
+        i{2} %% 2 = 0 /\
+        inzpRep4 f{1} = f{2}
+        ==>
+        inzpRep4 res{1} = zexp res{2} (exp 2 i1)
+    ].
+    move => *; proc *.
+    inline {1} 1. sp; wp.
+    call (eq_spec_impl__it_sqr_mulx i1 i2). skip => />.
+qed.
+
+
+lemma  eq_spec_impl_it_sqr_x2__mulx  (i1: int) (i2: int):
+    i1 = i2 => 2 <= i1 => i2 %% 2 = 0 =>
+    equiv[
+        M._it_sqr4_x2_ ~ CurveProcedures.it_sqr:
+        i1 = W32.to_uint i{1} /\
+        i2 = i{2}   /\
+        W32.to_uint i{1} = i{2} /\
+        i{2} %% 2 = 0 /\
+        inzpRep4 _f{1} = f{2}
+        ==>
+        inzpRep4 res{1} = zexp res{2} (exp 2 i1)
+    ].
+proof.
+    move => *; proc *.
+    inline{1} 1. inline{1} 5. wp; sp.
+    call (eq_spec_impl__it_sqr_mulx i1 i2). skip => />.
+qed.
+
+
+lemma eq_spec_impl_it_sqr_x2_mulx_x2 (i1: int) (i2: int):
+    2*i1 = i2 => 2 <= i1 => 4 <= i2 => i2 %% 2 = 0 =>
+equiv[
+        M._it_sqr4_x2 ~ CurveProcedures.it_sqr:
+       i1 = W32.to_uint i{1} /\
+        i2 = i{2}   /\
+        2*W32.to_uint i{1} = i{2} /\
+        i{2} %% 2 = 0 /\
+        inzpRep4 f{1} = f{2}
+        ==>
+        inzpRep4 res{1} = res{2}
+    ].
+    move => *; proc *.
+    inline {1} 1. sp; wp.
+    call (eq_spec_impl__it_sqr_mulx_x2 i1 i2). skip => />.
+qed.
+
+
+lemma  eq_spec_impl_it_sqr_x2__mulx_x2  (i1: int) (i2: int):
+    2*i1 = i2 => 2 <= i1 => 4 <= i2 => i2 %% 2 = 0 =>
+        equiv[
+        M._it_sqr4_x2_ ~ CurveProcedures.it_sqr:
+         i1 = W32.to_uint i{1} /\
+        i2 = i{2}   /\
+        2*W32.to_uint i{1} = i{2} /\
+        i{2} %% 2 = 0 /\
+        inzpRep4 _f{1} = f{2}
+        ==>
+        inzpRep4 res{1} = res{2}
+    ].
+proof.
+    move => *; proc *.
+    inline{1} 1. inline{1} 5. wp; sp.
+    call (eq_spec_impl__it_sqr_mulx_x2 i1 i2). skip => />.
+qed.
+
+
 (** step 9 : invert **)
-equiv eq_h4_invert :
-  MHop2.invert ~ M._fe64_invert : 
-     z1'{1} = inzpRep4 f{2}
+equiv eq_spec_impl_invert_mulx :
+  CurveProcedures.invert ~ M.__invert4:
+     fs{1} = inzpRep4 f{2}
   ==> res{1} = inzpRep4 res{2}.
 proof.
-proc.
-  call eq_h4_mul.
-  call eq_h4_sqr.
-  call eq_h4_it_sqr. wp.
-  call eq_h4_mul.
-  call eq_h4_it_sqr. wp.
-  call eq_h4_mul.
-  call eq_h4_it_sqr. wp.
-  call eq_h4_mul.
-  call eq_h4_it_sqr. wp.
-  call eq_h4_mul.
-  call eq_h4_it_sqr. wp.
-  call eq_h4_mul.
-  call eq_h4_it_sqr. wp.
-  call eq_h4_mul.
-  call eq_h4_it_sqr. wp.
-  call eq_h4_mul. wp.
-  call eq_h4_it_sqr. wp.
-  call eq_h4_sqr. wp.
-  call eq_h4_mul.
-  call eq_h4_sqr. wp.
-  call eq_h4_mul. wp.
-  call eq_h4_mul.
-  call eq_h4_sqr.
-  call eq_h4_sqr. wp.
-  call eq_h4_sqr. wp.
+proc. sp. auto => />.
+  call eq_spec_impl_mul_rsr__mulx. wp.
+  call eq_spec_impl_sqr_rr__mulx. wp.
+  symmetry;  call (eq_spec_impl_it_sqr_x2__mulx_x2 2 4); wp; symmetry.
+  call eq_spec_impl_mul_rsr__mulx. wp.
+  symmetry;  call (eq_spec_impl_it_sqr_x2__mulx_x2 25 50); wp; symmetry.
+  call eq_spec_impl_mul_rsr__mulx. wp.
+  symmetry;  call (eq_spec_impl_it_sqr_x2__mulx_x2 50 100); wp; symmetry.
+  call eq_spec_impl_mul_rsr__mulx. wp.
+  symmetry;  call (eq_spec_impl_it_sqr_x2__mulx_x2 25 50); wp; symmetry.
+  call eq_spec_impl_mul_rsr__mulx. wp.
+  symmetry;  call (eq_spec_impl_it_sqr_x2__mulx_x2 5 10); wp; symmetry.
+  call eq_spec_impl_mul_rsr__mulx. wp.
+  symmetry;  call (eq_spec_impl_it_sqr_x2__mulx_x2 10 20); wp; symmetry.
+  call eq_spec_impl_mul_rsr__mulx. wp.
+  symmetry;  call (eq_spec_impl_it_sqr_x2__mulx_x2 5 10); wp; symmetry.
+  call eq_spec_impl_mul_rsr__mulx. wp.
+  symmetry;  call (eq_spec_impl_it_sqr_x2__mulx_x2 2 4); wp; symmetry.
+  call eq_spec_impl_sqr_rr__mulx. wp.
+  call eq_spec_impl_mul_rsr__mulx. wp.
+  call eq_spec_impl_sqr_rr__mulx.  wp.
+  call eq_spec_impl_mul_rsr__mulx. wp.
+  call eq_spec_impl_mul_rsr__mulx. wp.
+  call eq_spec_impl_sqr_rr__mulx. wp.
+  call eq_spec_impl_sqr_rr__mulx. wp.
+  call eq_spec_impl_sqr_rr__mulx. wp. skip.  
   done.
 qed.
 
 (** step 10 : encode point **)
-equiv eq_h4_encode_point : 
-  MHop2.encode_point ~ M.encode_point:
-  true ==> true.
+equiv eq_spec_impl_encode_point_mulx : CurveProcedures.encode_point ~ M.__encode_point4:
+    x2{1}                 = inzpRep4 x2{2} /\
+    z2{1}                 = inzpRep4 z2r{2}
+    ==>
+    res{1} = pack4 (to_list  res{2}).
 proof.
-admit.
+    proc. wp.
+    ecall {2} (ph_to_bytes_mulx (r{2})). wp.
+    call eq_spec_impl_mul_rsr_mulx. wp.
+    call eq_spec_impl_invert_mulx.
+    wp; skip => />. move => H H0 H1.
+    by rewrite -H1.
 qed.
 
 (** step 11 : scalarmult **)
-equiv eq_h4_scalarmult :
-  MHop2.scalarmult ~ M._x25519_scalarmult:
-  true ==> true.
+equiv eq_spec_impl_scalarmult_internal_mulx :
+  CurveProcedures.scalarmult_internal ~ M.__curve25519_internal_mulx:
+        k'{1} = pack32 (to_list  k{2}) /\
+        u''{1} = inzpRep4 u{2}
+        ==>
+        res{1} = pack4 (to_list res{2}).
 proof.
-admit.
+    proc => /=. wp.
+    call eq_spec_impl_encode_point_mulx. wp.
+    call eq_spec_impl_montgomery_ladder_mulx. wp. skip.
+    done.
 qed.
+
+equiv eq_spec_impl_scalarmult_mulx :
+    CurveProcedures.scalarmult ~ M.__curve25519_mulx:
+        k'{1} = pack4 (to_list  _k{2}) /\
+        u'{1} = pack4 (to_list _u{2})
+        ==>
+        res{1} = pack4 (to_list res{2}).
+proof.
+    proc => /=. wp.
+    call eq_spec_impl_scalarmult_internal_mulx => />. wp.
+    call eq_spec_impl_decode_u_coordinate_mulx => />. wp.
+    call eq_spec_impl_decode_scalar_25519_mulx => />.
+    wp; skip => />.
+qed.
+
+equiv eq_spec_impl_scalarmult_base_mulx :
+    CurveProcedures.scalarmult_base ~ M.__curve25519_mulx_base:
+    k'{1} = pack4 (to_list  _k{2})
+    ==>
+    res{1} = pack4 (to_list res{2}).
+proof.
+    proc => /=; wp.
+    call eq_spec_impl_scalarmult_internal_mulx => />; wp.
+    call eq_spec_impl_decode_u_coordinate_base_mulx => />; wp.
+    call eq_spec_impl_decode_scalar_25519_mulx.
+    wp. skip => />.
+qed.
+
+lemma eq_spec_impl_scalarmult_jade_mulx _qp _np _pp:
+    equiv [CurveProcedures.scalarmult ~ M.jade_scalarmult_curve25519_amd64_mulx:
+        qp{2} = _qp                                                                              /\
+        np{2} = _np                                                                              /\
+        pp{2} = _pp                                                                              /\
+        k'{1} = pack4 (to_list np{2}) /\
+        u'{1} = pack4 (to_list  pp{2})
+        ==>
+        res{1} = pack4 (to_list res{2}.`1)     /\
+        res{2}.`2 = W64.zero].
+proof.
+    proc *. inline M.jade_scalarmult_curve25519_amd64_mulx; wp; sp.
+    call eq_spec_impl_scalarmult_mulx. skip => />.
+qed.
+
+lemma eq_spec_impl_scalarmult_jade_base  _qp _np:
+    equiv [CurveProcedures.scalarmult_base ~ M.jade_scalarmult_curve25519_amd64_mulx_base:
+        qp{2} = _qp                                                                              /\
+        np{2} = _np                                                                              /\
+        k'{1} = pack4 (to_list np{2})
+        ==>
+        res{1} = pack4 (to_list res{2}.`1)     /\
+        res{2}.`2 = W64.zero].
+proof.
+    proc *. inline M.jade_scalarmult_curve25519_amd64_mulx_base; wp; sp.
+    call eq_spec_impl_scalarmult_base_mulx. skip => />.
+qed.
+
+(* Proofs for older implementation *)
+(*
+lemma eq_spec_impl_scalarmult_jade_mulx mem _qp _np _pp:
+    equiv [CurveProcedures.scalarmult ~ M.jade_scalarmult_curve25519_amd64_mulx:
+        valid_ptr (W64.to_uint _qp)  32                                                          /\
+        valid_ptr (W64.to_uint _np)  32                                                          /\
+        valid_ptr (W64.to_uint _pp)  32                                                          /\
+        Glob.mem{2} = mem                                                                        /\
+        qp{2} = _qp                                                                              /\
+        np{2} = _np                                                                              /\
+        pp{2} = _pp                                                                              /\
+        k'{1} = pack4 (load_array4 (Glob.mem{2}) (W64.to_uint np{2})) /\
+        u'{1} = pack4 (load_array4 (Glob.mem{2}) (W64.to_uint pp{2}))
+        ==>
+        res{1} = pack4 (load_array4 Glob.mem{2} (W64.to_uint res{2}.`1))     /\
+        res{2}.`2 = W64.zero].
+proof.
+    proc *. inline M.jade_scalarmult_curve25519_amd64_mulx; wp; sp.
+    inline M.__load4 M.__store4.
+    do 3! unroll for{2} ^while. wp. sp.
+    call eq_spec_impl_scalarmult_mulx. skip => />.
+    move => &2 H H0 H1 H2 H3 H4.
+    do split.
+    congr; congr; rewrite  /load_array4 /to_list /mkseq -iotaredE => />.
+    do split.
+    congr; rewrite !to_uintD_small !to_uint_small => />. smt().
+    congr; rewrite !to_uintD_small !to_uint_small => />. smt().
+    congr; rewrite !to_uintD_small !to_uint_small => />. smt().
+    congr; congr; rewrite /load_array4 /to_list /mkseq -iotaredE => />.
+    do split.
+    congr; rewrite !to_uintD_small !to_uint_small => />. smt().
+    congr; rewrite !to_uintD_small !to_uint_small => />. smt().
+    congr; rewrite !to_uintD_small !to_uint_small => />. smt().
+    move => H5 H6 H7.
+    congr; rewrite /load_array4 /to_list /mkseq -iotaredE => />.
+    congr; congr.
+    apply (load_store_pos Glob.mem{2} qp{2} H7 0). rewrite /valid_ptr; by do split => /> //=. done.
+    congr.
+    apply (load_store_pos Glob.mem{2} qp{2} H7 8). rewrite /valid_ptr; by do split => /> //=. done.
+    congr.
+    apply (load_store_pos Glob.mem{2} qp{2} H7 16). rewrite /valid_ptr; by do split => /> //=. done.
+    congr.
+    apply (load_store_pos Glob.mem{2} qp{2} H7 24). rewrite /valid_ptr; by do split => /> //=. done.
+qed.
+*)
+
+(*
+lemma eq_spec_impl_scalarmult_jade_base  mem _qp _np:
+    equiv [CurveProcedures.scalarmult_base ~ M.jade_scalarmult_curve25519_amd64_mulx_base:
+        valid_ptr (W64.to_uint _qp)  32                                                          /\
+        valid_ptr (W64.to_uint _np)  32                                                          /\
+        Glob.mem{2} = mem                                                                        /\
+        qp{2} = _qp                                                                              /\
+        np{2} = _np                                                                              /\
+        k'{1} = pack4 (load_array4 (Glob.mem{2}) (W64.to_uint np{2}))
+        ==>
+        res{1} = pack4 (load_array4 Glob.mem{2} (W64.to_uint res{2}.`1))     /\
+        res{2}.`2 = W64.zero].
+proof.
+    proc *. inline M.jade_scalarmult_curve25519_amd64_mulx_base. wp. sp.
+    inline M.__load4 M.__store4.
+    do 2! unroll for{2} ^while. wp; sp.
+    call eq_spec_impl_scalarmult_base_mulx. skip  => />.
+    move => &2 H H0 H1 H2. do split.
+    congr; congr; rewrite  /load_array4 /to_list /mkseq -iotaredE => />.
+    do split.
+    congr; rewrite !to_uintD_small !to_uint_small => />. smt().
+    congr; rewrite !to_uintD_small !to_uint_small => />. smt().
+    congr; rewrite !to_uintD_small !to_uint_small => />. smt().
+    move => H3 H4.
+    congr; congr; rewrite /load_array4 /to_list /mkseq -iotaredE => />.
+    do split.
+    apply (load_store_pos Glob.mem{2} qp{2} H4 0). rewrite /valid_ptr; by do split => /> //=. done.
+    apply (load_store_pos Glob.mem{2} qp{2} H4 8). rewrite /valid_ptr; by do split => /> //=. done.
+    apply (load_store_pos Glob.mem{2} qp{2} H4 16). rewrite /valid_ptr; by do split => /> //=. done.
+    apply (load_store_pos Glob.mem{2} qp{2} H4 24). rewrite /valid_ptr; by do split => /> //=. done.
+qed.
+*)
